

Ejercicio en Clase

x	F(x)
1	0
4	1.386294
5	1.609438
6	1.791752

Evaluar $F(2)$ usando la interpolación lineal, cuadrática y cúbica

Interpolación lineal

$$F(x) = \frac{F(x_1) - F(x_0)}{x_1 - x_0} (x - x_0) + F(x_0)$$

$$F(2) = \frac{1.386294 - 0}{4 - 1} (2 - 1) + 0 = 0.462098$$

Interpolación cuadrática

$$F(x) = F(x_0) + \left(\frac{F(x_1) - F(x_0)}{x_1 - x_0} \right) (x - x_0) + \left(\frac{F(x_2) - F(x_1)}{x_2 - x_1} - \frac{F(x_1) - F(x_0)}{x_1 - x_0} \right) \frac{(x - x_0)^2}{(x_1 - x_0)}$$

$$F(2) = 0 + \left(\frac{1.386294 - 0}{4 - 1} \right) (2 - 1) + \left(\frac{1.609438 - 1.386294}{5 - 4} - \frac{1.386294 - 0}{4 - 1} \right) \frac{(2 - 1)^2}{5 - 1}$$

$$F(2) = 0.462098 + \left(\frac{0.223144 - 0.462098}{5 - 1} \right) * (-2)$$

$$F(2) = 0.581575$$

Interpolación Polinomial

$$F_3(x) = F(x_0) + (x-x_0) \frac{F(x_1) - F(x_0)}{x_1 - x_0} + (x-x_0)(x-x_1) \frac{F(x_2) - F(x_1)}{x_2 - x_1 - \frac{F(x_1) - F(x_0)}{x_1 - x_0} (x_2 - x_0)} + (x-x_0)(x-x_1)(x-x_2) \frac{F(x_3) - F(x_2)}{x_3 - x_2 - \frac{F(x_2) - F(x_1)}{x_2 - x_1} (x_3 - x_0) - \frac{F(x_1) - F(x_0)}{x_1 - x_0} (x_3 - x_2)}$$

$$F_3(x) = 0.581576 + (2-1)(2-4)(2-6) \frac{(1.791752 - 1.609438)}{6-6}$$

$$- \frac{(1.609438 - 1.386294)}{6-4}$$

$$- \frac{1.386294 - 0}{4-1}$$

$$F_3(x) = 0.676616$$